spi_abs/spi_absstateScript.sml
@@ -1,0 +1,55 @@
+open HolKernel bossLib boolLib Parse;
+open wordsLib wordsTheory;
+open SPI_stateTheory;
+
+(* SPI_abs model states *)
+val _ = new_theory "spi_absstate";
+
+(* spi_abs controller initialization automaton *)
+val _ = Datatype `abs_init_general_state = 
+| abs_init_start | abs_init_setregs | abs_init_done`
+
+val _ = Datatype `abs_init_state = <|
+state: abs_init_general_state;
+sysconfig_mode_done: bool;
+modulctrl_bus_done: bool;
+ch0conf_wordlen_done: bool;
+ch0conf_mode_done: bool;
+ch0conf_speed_done: bool |>`
+
+(* spi_abs controller transmit automaton *)
+val _ = Datatype `abs_tx_general_state =
+| abs_tx_idle | abs_tx_conf_ready | abs_tx_ready_for_trans
+| abs_tx_trans_done | abs_tx_channel_disabled`
+
+val _ = Datatype `abs_tx_state = <|
+state: abs_tx_general_state |>`
+
+(* spi_abs controller receive automaton *)
+val _ = Datatype `abs_rx_general_state =
+| abs_rx_idle | abs_rx_conf_ready | abs_rx_receive_data 
+| abs_rx_data_ready | abs_rx_channel_disabled`
+
+val _ = Datatype `abs_rx_state = <|
+state: abs_rx_general_state |>`
+
+(* spi_abs controller transfer automaton (full-dulplex mode) *)
+val _ = Datatype `abs_xfer_general_state =
+| abs_xfer_idle | abs_xfer_conf_ready | abs_xfer_ready_for_trans
+| abs_xfer_exchange_data | abs_xfer_data_ready | abs_xfer_channel_disabled`
+
+val _ = Datatype `abs_xfer_state = <|
+state : abs_xfer_general_state |>`
+
+(* spi_abs controller model state*)
+val _ = Datatype `spi_abs_state = <|
+err: bool;
+regs: spi_regs;
+TX_SHIFT_REG : word8;
+RX_SHIFT_REG : word8;
+init: abs_init_state;
+tx: abs_tx_state;
+rx: abs_rx_state;
+xfer: abs_xfer_state |>`
+
+val _ = export_theory();
