spi_model/SPI_schedulerScript.sml
@@ -18,7 +18,10 @@ TX_ENABLE (spi:spi_state) =
 (spi.tx.state <> tx_conf_ready) /\ 
 (spi.tx.state <> tx_ready_for_trans) /\ 
 (spi.tx.state <> tx_trans_done) /\ 
-(spi.tx.state <> tx_channel_disabled))`
+(spi.tx.state <> tx_channel_disabled) /\
+(spi.init.state = init_done) /\
+(spi.rx.state = rx_idle) /\
+(spi.xfer.state = xfer_idle))`
 
 val RX_ENABLE_def = Define `
 RX_ENABLE (spi:spi_state) =
@@ -26,7 +29,10 @@ RX_ENABLE (spi:spi_state) =
 (spi.rx.state <> rx_conf_ready) /\ 
 (spi.rx.state <> rx_receive_data) /\
 (spi.rx.state <> rx_data_ready) /\ 
-(spi.rx.state <> rx_channel_disabled))`
+(spi.rx.state <> rx_channel_disabled) /\
+(spi.init.state = init_done) /\
+(spi.tx.state = tx_idle) /\
+(spi.xfer.state = xfer_idle))`
 
 val XFER_ENABLE_def = Define `
 XFER_ENABLE (spi:spi_state) =
@@ -35,8 +41,12 @@ XFER_ENABLE (spi:spi_state) =
 (spi.xfer.state <> xfer_ready_for_trans) /\
 (spi.xfer.state <> xfer_exchange_data) /\ 
 (spi.xfer.state <> xfer_data_ready) /\ 
-(spi.xfer.state <> xfer_channel_disabled))`
+(spi.xfer.state <> xfer_channel_disabled) /\
+(spi.init.state = init_done) /\
+(spi.tx.state = tx_idle) /\
+(spi.rx.state = rx_idle))`
 
+(* not used so far
 (* sheduler_cases: schedule -> spi_state -> spi_state *)
 val scheduler_cases_def = Define `
 (scheduler_cases Initialize (spi:spi_state) = 
@@ -54,5 +64,6 @@ spi_scheduler (env:environment) (spi:spi_state) =
 if spi.err then spi
 else 
 scheduler_cases env.scheduler spi`
+*)
 
 val _ = export_theory();
