thm/spi_abs_preserves_invScript.sml
@@ -1,0 +1,28 @@
+open HolKernal bossLib boolLib Parse;
+open wordsLib wordsTHeory;
+open abs_invTheory;
+
+val _ = new_theory "spi_abs_preserves_inv"
+
+
+
+
+
+
+
+
+
+
+
+
+
+
+(* fianl goal for invariant proof *)
+val spi_abs_preserves_invariant = store_thm("spi_abs_preserves_invariant",
+``!spi_abs l. (spi_abs_invariant spi_abs) /\ (spi_abs_tr spi_abs l spi_abs') 
+==> (spi_abs_invariant spi_abs')``,
+cheat);
+
+
+
+val _ = new_theory();
