spi_abs/readme.md
@@ -1,7 +1,7 @@
 The refinement of SPI controller model
 
 ### Description
-Based on the spi controller model we defined in the folder /spi_model, we build an abstract spi controller model `spi_ref`. 
+Based on the spi controller model we defined in folder spi_model, we build an abstract spi controller model `spi_ref`. 
 
 It removes most internal operations of SPI, to simplify the model. This model contains an update function `write_refregs`, a return function `read_refregs`, as well as 3 label functions for `TX`, `RX` and `XFER` respectively. 
 Therefore, this model can update itself when driver issue write commands, or return a register's value and update its state for read commands, and more importandly, perform data transition with another spi device using `TX`, `RX` or `XFER` mode. 
@@ -10,7 +10,7 @@ The behaviors of the abstract model and the baisc one, from the driver angle, ar
 ### Files
 - `spi_refstateScript.sml`: define the datatypes of the `spi_ref` model, mainly remove some internal states of spi automatons.
 
-- `write_refregsScript.sml`: define write-related functions that shows how the `spi_ref` updates itself according to the driver write commands.
+- `write_refregsScript.sml`: define write-related functions, that shows how the `spi_ref` update itself according to the driver write commands.
 
 - `read_refregsScript.sml`: define read-related functions for read commands.
 
